icing/examples/dopplerProgErrorScript.sml
@@ -22,5 +22,47 @@ Theorem errorbounds_AST =
   EVAL (Parse.Term
        ‘isOkError ^(concl theAST_opt |> rhs) doppler_pre theErrBound’);
 
+Theorem errorbound_opt =
+  EVAL (Parse.Term
+       ‘getError ^(concl theAST_opt |> rhs) doppler_pre theErrBound’);
+
+val doppler_unopt =
+“[Dlet unknown_loc (Pvar "doppler")
+ (Fun "u" (Fun "v" (Fun "t"
+  (** Numerical kernel **)
+  (FpOptimise NoOpt
+   (Let (SOME "t1")
+    (App (FP_bop FP_Add)
+     [
+       (App FpFromWord [Lit (Word64 (4644537666646730342w:word64))]);
+       (App (FP_bop FP_Mul)
+        [
+          (App FpFromWord [Lit (Word64 (4603579539098121011w:word64))]);
+          Var (Short  "t")
+        ])
+     ])
+    (App (FP_bop FP_Div)
+     [
+       (App (FP_bop FP_Mul)
+        [
+          (App (FP_uop FP_Neg)
+           [Var (Short "t1")]);
+          Var (Short "v")
+        ]);
+       (App (FP_bop FP_Mul)
+        [
+          (App (FP_bop FP_Add)
+           [Var (Short "t1");
+            Var (Short "u")]);
+          (App (FP_bop FP_Add)
+           [Var (Short "t1");
+            Var (Short "u")])
+        ])
+     ])
+     )))))]”;
+
+Theorem errorbound_unopt =
+  EVAL (Parse.Term
+       ‘getError ^(doppler_unopt) doppler_pre theErrBound’);
 
 val _ = export_theory();
