icing/examples/nn1LayerProgErrorScript.sml
@@ -22,4 +22,91 @@ Theorem errorbounds_AST =
   EVAL (Parse.Term
        ‘isOkError ^(concl theAST_opt |> rhs) nn1Layer_pre theErrBound’);
 
+Theorem errorbound_opt =
+  EVAL (Parse.Term
+       ‘getError ^(concl theAST_opt |> rhs) nn1Layer_pre theErrBound’);
+
+val nn1Layer =
+(** REPLACE AST BELOW THIS LINE **)
+“[
+Dlet unknown_loc (Pvar "nn1Layer")
+(Fun "x1" (Fun "x2" (Fun "x3" (Fun "x4" (FpOptimise NoOpt
+(Let (SOME "dot1")
+  (App (FP_bop FP_Add)
+    [
+      (App (FP_bop FP_Sub)
+      [
+        (App (FP_bop FP_Sub)
+        [
+          (App (FP_bop FP_Sub)
+          [
+            (App (FP_bop FP_Mul)
+            [
+              (App FpFromWord [Lit (Word64 (-4623678203515150061w:word64))]);
+              Var (Short  "x1")
+            ]);
+            (App (FP_bop FP_Mul)
+            [
+              (App FpFromWord [Lit (Word64 (4599812728369788328w:word64))]);
+              Var (Short  "x2")
+            ])
+          ]);
+          (App (FP_bop FP_Mul)
+          [
+            (App FpFromWord [Lit (Word64 (4614369037905393877w:word64))]);
+            Var (Short  "x3")
+          ])
+        ]);
+        (App (FP_bop FP_Mul)
+        [
+          (App FpFromWord [Lit (Word64 (4609904394414800136w:word64))]);
+          Var (Short  "x4")
+        ])
+      ]);
+      (App FpFromWord [Lit (Word64 (4598694034222349497w:word64))])
+    ])
+  (Let (SOME "dot2")
+    (App (FP_bop FP_Add)
+      [
+        (App (FP_bop FP_Sub)
+        [
+          (App (FP_bop FP_Add)
+          [
+            (App (FP_bop FP_Add)
+            [
+              (App (FP_bop FP_Mul)
+              [
+                (App FpFromWord [Lit (Word64 (-4629260865613238528w:word64))]);
+                Var (Short  "x1")
+              ]);
+              (App (FP_bop FP_Mul)
+              [
+                (App FpFromWord [Lit (Word64 (4593826543745087465w:word64))]);
+                Var (Short  "x2")
+              ])
+            ]);
+            (App (FP_bop FP_Mul)
+            [
+              (App FpFromWord [Lit (Word64 (4615768531489599259w:word64))]);
+              Var (Short  "x3")
+            ])
+          ]);
+          (App (FP_bop FP_Mul)
+          [
+            (App FpFromWord [Lit (Word64 (4611127572073593962w:word64))]);
+            Var (Short  "x4")
+          ])
+        ]);
+        (App FpFromWord [Lit (Word64 (4598685027023094756w:word64))])
+      ])
+    (App (FP_bop FP_Sub)
+      [
+        Var (Short  "dot1");
+        Var (Short  "dot2")
+      ]))))))))]”;
+
+Theorem errorbound_unopt =
+  EVAL (Parse.Term
+       ‘getError ^nn1Layer nn1Layer_pre theErrBound’);
+
 val _ = export_theory();
